<?xml version="1.0" encoding="utf-8"?>
<rdf:RDF
  xmlns:rdfs="http://www.w3.org/2000/01/rdf-schema#"
  xmlns:rdf="http://www.w3.org/1999/02/22-rdf-syntax-ns#"
  xmlns:owl="http://www.w3.org/2002/07/owl#"
  xmlns:dcterms="http://purl.org/dc/terms/"
>
  <owl:Ontology rdf:about="https://w3id.org/inspec/datavoc/">
    <rdfs:label xml:lang="en">The Interoperable Specifications Profile (INSPEC) Vocabulary</rdfs:label>
    <rdfs:comment xml:lang="en">This vocabulary defines terms used in INSPEC.</rdfs:comment>
  </owl:Ontology>
  <dcterms:Standard rdf:about="https://w3id.org/inspec/datavoc/PROF">
    <rdfs:label xml:lang="en">PROF</rdfs:label>
    <rdfs:isDefinedBy rdf:resource="https://w3id.org/inspec/datavoc/"/>
    <rdfs:comment xml:lang="en">This is a specification corresponding to a profile of PROF used to capture an interoperable specification. Corresponds to the rules INSPEC-1 — INSPEC-10.</rdfs:comment>
    <rdfs:seeAlso rdf:resource="https://www.w3.org/TR/dx-prof/"/>
  </dcterms:Standard>
  <dcterms:Standard rdf:about="https://w3id.org/inspec/datavoc/RDFS">
    <rdfs:label xml:lang="en">RDFS</rdfs:label>
    <rdfs:isDefinedBy rdf:resource="https://w3id.org/inspec/datavoc/"/>
    <rdfs:comment xml:lang="en">This is a specification corresponding to a profile of RDFS used to capture an expression of data vocabularies. Corresponds to the rules DV-1 — DV-6.</rdfs:comment>
    <rdfs:seeAlso rdf:resource="https://www.w3.org/TR/rdf12-schema/"/>
  </dcterms:Standard>
  <dcterms:Standard rdf:about="https://w3id.org/inspec/datavoc/SKOS">
    <rdfs:label xml:lang="en">SKOS</rdfs:label>
    <rdfs:isDefinedBy rdf:resource="https://w3id.org/inspec/datavoc/"/>
    <rdfs:comment xml:lang="en">This is a specification corresponding to a profile of SKOS used to capture an expression of terminologies. Corresponds to the rules TE-1 — TE-5.</rdfs:comment>
    <rdfs:seeAlso rdf:resource="https://www.w3.org/TR/skos-reference/"/>
  </dcterms:Standard>
  <dcterms:Standard rdf:about="https://w3id.org/inspec/datavoc/SHACL">
    <rdfs:label xml:lang="en">SHACL</rdfs:label>
    <rdfs:isDefinedBy rdf:resource="https://w3id.org/inspec/datavoc/"/>
    <rdfs:comment xml:lang="en">This is a specification corresponding to a profile of SHACL used to capture an expression of application profiles. Corresponds to the rules AP-1 — AP-14.</rdfs:comment>
    <rdfs:seeAlso rdf:resource="https://www.w3.org/TR/shacl"/>
  </dcterms:Standard>
  <dcterms:Standard rdf:about="https://w3id.org/inspec/datavoc/SVG">
    <rdfs:label xml:lang="en">SVG</rdfs:label>
    <rdfs:isDefinedBy rdf:resource="https://w3id.org/inspec/datavoc/"/>
    <rdfs:comment xml:lang="en">This is a specification corresponding to a profile of SVG used to capture an expression of diagrams for interoperable specifications. Corresponds to the rules SVG-1 — SVG-5.</rdfs:comment>
    <rdfs:seeAlso rdf:resource="https://www.w3.org/TR/SVG11/"/>
  </dcterms:Standard>
  <rdf:Property rdf:about="https://w3id.org/inspec/datavoc/variant">
    <rdfs:label xml:lang="en">variant</rdfs:label>
    <rdfs:isDefinedBy rdf:resource="https://w3id.org/inspec/datavoc/"/>
    <rdfs:comment xml:lang="en">A shape or profile is a variant of another if it relaxes some of its constraints</rdfs:comment>
    <rdfs:subPropertyOf rdf:resource="http://purl.org/dc/terms/relation"/>
    <rdfs:domain>
      <rdf:Description rdf:nodeID="naf255206f4f948d1bb5e5f5f0440d55db1">
        <owl:unionOf rdf:parseType="Collection">
          <rdf:Description rdf:about="http://www.w3.org/ns/shacl#Shape"/>
          <rdf:Description rdf:about="http://www.w3.org/ns/dx/prof/Profile"/>
        </owl:unionOf>
      </rdf:Description>
    </rdfs:domain>
    <rdfs:range>
      <rdf:Description rdf:nodeID="naf255206f4f948d1bb5e5f5f0440d55db4">
        <owl:unionOf rdf:parseType="Collection">
          <rdf:Description rdf:about="http://www.w3.org/ns/shacl#Shape"/>
          <rdf:Description rdf:about="http://www.w3.org/ns/dx/prof/Profile"/>
        </owl:unionOf>
      </rdf:Description>
    </rdfs:range>
  </rdf:Property>
  <rdf:Property rdf:about="https://w3id.org/inspec/datavoc/refines">
    <rdfs:label xml:lang="en">refines</rdfs:label>
    <rdfs:isDefinedBy rdf:resource="https://w3id.org/inspec/datavoc/"/>
    <rdfs:comment xml:lang="en">A shape refines another by adding additional constraints to it</rdfs:comment>
    <rdfs:subPropertyOf rdf:resource="http://purl.org/dc/terms/relation"/>
    <rdfs:domain rdf:resource="http://www.w3.org/ns/shacl#Shape"/>
    <rdfs:range rdf:resource="http://www.w3.org/ns/shacl#Shape"/>
    <rdfs:seeAlso rdf:resource="http://www.w3.org/ns/dx/prof/isProfileOf"/>
  </rdf:Property>
  <rdf:Property rdf:about="https://w3id.org/inspec/datavoc/reuses">
    <rdfs:label xml:lang="en">reuses</rdfs:label>
    <rdfs:isDefinedBy rdf:resource="https://w3id.org/inspec/datavoc/"/>
    <rdfs:comment xml:lang="en">A specification reuses a resource if it is needed by the specification but was originally introduced by a different specification</rdfs:comment>
    <rdfs:subPropertyOf rdf:resource="http://purl.org/dc/terms/relation"/>
    <rdfs:domain rdf:resource="http://purl.org/dc/terms/Standard"/>
    <rdfs:range rdf:resource="http://www.w3.org/2000/01/rdf-schema#Resource"/>
  </rdf:Property>
  <rdf:Property rdf:about="https://w3id.org/inspec/datavoc/introduces">
    <rdfs:label xml:lang="en">introduces</rdfs:label>
    <rdfs:isDefinedBy rdf:resource="https://w3id.org/inspec/datavoc/"/>
    <rdfs:comment xml:lang="en">A specification introduces a resource if it is first introduced by a the same specification</rdfs:comment>
    <rdfs:subPropertyOf rdf:resource="http://purl.org/dc/terms/relation"/>
    <rdfs:domain rdf:resource="http://purl.org/dc/terms/Standard"/>
    <rdfs:range rdf:resource="http://www.w3.org/2000/01/rdf-schema#Resource"/>
  </rdf:Property>
</rdf:RDF>
